\section{Simple series}

\begin{center}
\begin{tabular}{ccc}
\hline
\hline
$\sum\limits_{i=1}^{n} i  $ & $=$ & $\frac{n(n+1)}{2}$ \\
\hline
$\sum\limits_{i=1}^{n} i^2$ & $=$ & $\frac{n(n+1)(2n + 1)}{6}$ \\
\hline
$\sum\limits_{i=1}^{n} i^3$ & $=$ & $\frac{n^2(n+1)^2}{4}$ \\
\hline
\hline
$\sum\limits_{i = 1}^n r^i$ & $=$ & $\frac{1-r^n}{1-r}$\\ 
\hline
$\sum\limits_{i = 1}^\infty r^i$ & $=$ & $\frac{1}{1-r}$\\ 
\hline
$\sum\limits_{i = 1}^\infty i \cdot r^i$ & $=$ & $\frac{r}{(1-r)^2}$\\ 
\hline
$\sum\limits_{i = 1}^\infty i^2 \cdot r^i$ & $=$ & $\frac{r\cdot(r+1)}{(1-r)^3}$\\ 
\hline
\hline
\end{tabular}
\end{center}
